client.v
@@ -1,16 +1,42 @@
 Require Import ZArith.
 Require Import String.
 
-Require Import packet.
+AddPath "/Users/joald/wwk/client" as.
 
-Inductive mode : Set := Read | Write.
+Load packet.
 
-Record init_state : Set := mkState {
-    transfer_mode : mode;
-    filename : string;
-    port: positive;
-    last_packet : option packet;
-    timeout_count : N;
+Record state : Set := mkState {
+  transfer_mode : mode;
+  port: option positive;
+  last_packet : option packet;
+  timeout_count : N;
+  file_contents : string;
 }.
+
+(*
+Inductive packet : Set := 
+| p_RRQ : string -> packet                  (* Filename *)
+| p_WRQ : string -> packet                  (* Filename *)
+| p_DATA : forall (x : N), x < two_bytes_range_size -> string -> packet     (* Block #, Data *)
+| p_ACK : forall (x : N), x < two_bytes_range_size -> packet                (* Block # *)
+| p_ERROR : error_code -> string -> packet. (* ErrorCode, ErrMsg *)
+*)
+
+Record result := mkResult {
+  packet_to_send : option packet;
+  new_state : option state;
+  file_data : option string;
+}.
+
+(** When reading:
+  - in_file is the name of the file on the server.
+  - out_file is the name of the file on the local machine.
+  When writing:
+  - in_file is the contents of the file on the local machine.
+  - out_file is the name of the file on the server
+*)
+Definition coq_init (rw_mode : mode) (in_file : string) (out_file : string) : result := 
+  (serialize_packet (init_packet mode in_file out_file), 
+   mkState mode None None (?) match
 
 Definition coq_process_state () := .
